forall_inst step_checker

src/spl/Assumptions.v
@@ -30,7 +30,7 @@ Section Interp_UF.
   Fixpoint interp_uf (rho:Valuation.t) (c:C.t) :=
     match c with
     | nil => false
-    | l::nil => Lit.interp rho l
+    | l::nil => Lit.interp rho l 
     | l::c => (Lit.interp rho l) || (interp_uf rho c)
     end.
 
@@ -65,10 +65,10 @@ Section Checker.
       | x::xs, y::ys => (P x y) && (forallb2 xs ys)
       | _, _ => false
       end.
-
+ 
   End Forallb2.
 
-  Definition check_hole (s:S.t) (prem_id:list clause_id) (prem:list C.t) (concl:C.t) :=
+  Definition check_hole (s:S.t) (prem_id:list clause_id) (prem:list C.t) (concl:C.t) : C.t :=
     if forallb2 (fun id c => forallb2 (fun i j => i == j) (S.get s id) (S.sort_uniq c)) prem_id prem
     then concl
     else C._true.
@@ -116,17 +116,15 @@ Section Checker_correct.
 
   Lemma valid_check_hole: C.valid rho (check_hole s prem_id prem concl).
   Proof.
-    unfold check_hole. revert prem p. induction prem_id as [ |pid pids IHpids]; simpl;
+    unfold check_hole. revert prem p.
+    induction prem_id as [ |pid pids IHpids]; simpl;
       intros [ |p ps]; simpl; intro H.
     - unfold C.valid. now rewrite interp_equiv.
     - now apply C.interp_true.
     - now apply C.interp_true.
     - case_eq (forallb2 (fun i j => i == j) (S.get s pid) (S.sort_uniq p));
       simpl; intro Heq; [ |now apply C.interp_true].
-      case_eq (forallb2 (fun id c => forallb2 (fun i j => i == j) (S.get s id) (S.sort_uniq c)) pids ps);
-      simpl; intro Heq2; [ |now apply C.interp_true].
-      assert (IH:=IHpids _ (H (valid_check_clause _ _ Heq))).
-      now rewrite Heq2 in IH.
+      apply IHpids. apply H. apply (valid_check_clause _ _ Heq).
   Qed.
 
 End Checker_correct.
