src/Trace.v
@@ -16,7 +16,8 @@
 
 Require Import Bool Int63 PArray.
 Require Structures.
-Require Import Misc State SMT_terms Cnf Euf Lia Syntactic Arithmetic Operators Assumptions.
+(* attention *)
+Require Import SMTCoq.Misc SMTCoq.State SMTCoq.SMT_terms Cnf Euf Lia Syntactic Arithmetic Operators Assumptions.
 
 Local Open Scope array_scope.
 Local Open Scope int63_scope.
@@ -317,6 +318,7 @@ Module Euf_Checker.
   Variable t_atom : array Atom.atom.
   Variable t_form : array Form.form.
 
+  
   Inductive step :=
   | Res (pos:int) (res:resolution)
   | ImmFlatten (pos:int) (cid:clause_id) (lf:_lit)
@@ -339,8 +341,9 @@ Module Euf_Checker.
      WARNING: this breaks extraction. *)
   | Hole (pos:int) (prem_id:list clause_id) (prem:list C.t) (concl:C.t)
     (p:interp_conseq_uf (Form.interp_state_var (Atom.interp_form_hatom t_i t_func t_atom) t_form) prem concl)
-  .
-
+  | ForallInst (pos:int) (lemma:Prop) (pl:lemma) (concl:C.t)
+    (p: lemma -> interp_conseq_uf (Form.interp_state_var (Atom.interp_form_hatom t_i t_func t_atom) t_form) nil concl).
+  
   Local Open Scope list_scope.
 
   Local Notation check_flatten t_atom t_form := (check_flatten t_form (check_hatom t_atom) (check_neg_hatom t_atom)) (only parsing).
@@ -365,8 +368,9 @@ Module Euf_Checker.
       | SplArith pos orig res l => S.set_clause s pos (check_spl_arith t_form t_atom (S.get s orig) res l)
       | SplDistinctElim pos orig res => S.set_clause s pos (check_distinct_elim t_form t_atom (S.get s orig) res)
       | @Hole pos prem_id prem concl _ => S.set_clause s pos (check_hole s prem_id prem concl)
+      | ForallInst pos lemma _ concl  _ => S.set_clause s pos concl
     end.
-
+  
   Lemma step_checker_correct :
     let rho := Form.interp_state_var (Atom.interp_form_hatom t_i t_func t_atom) t_form in
       Form.check_form t_form -> Atom.check_atom t_atom ->
@@ -374,7 +378,7 @@ Module Euf_Checker.
       forall s, S.valid rho s ->
         forall st : step, S.valid rho (step_checker s st).
   Proof.
-    intros rho H1 H2 H10 s Hs. destruct (Form.check_form_correct (Atom.interp_form_hatom t_i t_func t_atom) _ H1) as [[Ht1 Ht2] Ht3]. destruct (Atom.check_atom_correct _ H2) as [Ha1 Ha2]. intros [pos res|pos cid lf|pos|pos|pos l|pos l|pos l i|pos cid|pos cid|pos cid i|pos l fl|pos l fl|pos l1 l2 fl|pos cl c|pos l|pos orig res l|pos orig res|pos prem_id prem concl p]; simpl; try apply S.valid_set_clause; auto.
+    intros rho H1 H2 H10 s Hs. destruct (Form.check_form_correct (Atom.interp_form_hatom t_i t_func t_atom) _ H1) as [[Ht1 Ht2] Ht3]. destruct (Atom.check_atom_correct _ H2) as [Ha1 Ha2]. intros [pos res|pos cid lf|pos|pos|pos l|pos l|pos l i|pos cid|pos cid|pos cid i|pos l fl|pos l fl|pos l1 l2 fl|pos cl c|pos l|pos orig res l|pos orig res|pos prem_id prem concl p | ]; simpl; try apply S.valid_set_clause; auto.
     apply S.valid_set_resolve; auto.
     apply valid_check_flatten; auto; intros h1 h2 H.
     rewrite (Syntactic.check_hatom_correct_bool _ _ _ Ha1 Ha2 _ _ H); auto.
@@ -395,6 +399,11 @@ Module Euf_Checker.
     apply valid_check_spl_arith; auto.
     apply valid_check_distinct_elim; auto.
     apply valid_check_hole; auto.
+
+    intros pos lemma pl concl l. fold rho in l.
+    apply S.valid_set_clause; auto.
+    unfold C.valid. rewrite interp_equiv.
+    now apply l. 
   Qed.
 
   Definition euf_checker (* t_atom t_form *) s t :=
@@ -476,6 +485,7 @@ Module Euf_Checker.
     end &&
     let (nclauses,_,_) := c in
     checker (* t_i t_func t_atom t_form *) (PArray.make nclauses l) None c.
+
 
   Lemma checker_eq_correct : forall (* t_i t_func t_atom t_form *) l1 l2 l c,
     checker_eq (* t_func t_atom t_form *) l1 l2 l c = true ->
